Weidenbach_Book/IsaSAT/Pairing_Heaps_Impl_LLVM.thy
@@ -339,4 +339,5 @@ lemmas [sepref_fr_rules] =
   mop_vsids_pop_min2_impl_code.refine[FCOMP mop_vsids_pop_min2_impl2, FCOMP vsids_pop_min2_mop_prio_pop_min2]
   mop_hp_read_score_imp_code.refine[FCOMP mop_hp_read_score_imp_mop_hp_read_score2, FCOMP mop_hp_read_score_mop_prio_old_weight2]
 
+
 end
